src/program_proof/pav/server.v
@@ -1,7 +1,7 @@
 From Perennial.program_proof Require Import grove_prelude.
 From Goose.github_com.mit_pdos.pav Require Import kt.
 
-From Perennial.program_proof.pav Require Import cryptoffi.
+From Perennial.program_proof.pav Require Import core cryptoffi serde.
 
 Section inv.
 Context `{!heapGS Σ}.
@@ -19,8 +19,37 @@ Definition own (ptr : loc) (obj : t) : iProp Σ. Admitted.
 End defs.
 End Server.
 
-Section specs.
+Section wps.
 Context `{!heapGS Σ}.
+Lemma wp_compMapVal (epoch : w64) ptr_pk_open pk_open :
+  {{{
+    "Hown_pk_open" ∷ CommitOpen.own ptr_pk_open pk_open
+  }}}
+  compMapVal #epoch #ptr_pk_open
+  {{{
+    sl_map_val commit, RET (slice_val sl_map_val);
+    "Hown_pk_open" ∷ CommitOpen.own ptr_pk_open pk_open ∗
+    "#His_commit" ∷ is_commit pk_open.(CommitOpen.Val) commit ∗
+    "Hsl_map_val" ∷ own_slice_small sl_map_val byteT (DfracOwn 1)
+      (MapValPre.encodesF (MapValPre.mk epoch commit))
+  }}}.
+Proof.
+  iIntros (Φ) "H HΦ". iNamed "H". wp_rec.
+  wp_apply wp_NewSlice_0. iIntros "* Hsl_enc".
+  wp_apply (CommitOpen.wp_enc with "[$Hsl_enc $Hown_pk_open]").
+  iIntros "*". iNamedSuffix 1 "_open". simpl.
+  iDestruct (own_slice_to_small with "Hsl_enc_open") as "Hsl_enc_open".
+  wp_apply (wp_Hash with "[$Hsl_enc_open]"). iIntros "*". iNamed 1.
+  wp_apply wp_allocStruct; [val_ty|]. iIntros "* H".
+  iDestruct (struct_fields_split with "H") as "H". iNamed "H".
+  wp_apply wp_NewSlice_0. iIntros "* Hsl_enc".
+  iMod (own_slice_small_persist with "Hhash") as "#Hhash".
+  wp_apply (MapValPre.wp_enc (MapValPre.mk _ _) with "[$Hsl_enc $Epoch $PkCommit $Hhash]").
+  iIntros "*". iNamedSuffix 1 "_mapval". simpl.
+  iDestruct (own_slice_to_small with "Hsl_enc_mapval") as "Hsl_enc_mapval".
+  iApply "HΦ". iFrame "∗#".
+Qed.
+
 Lemma wp_newServer :
   {{{ True }}}
   NewServer #()
@@ -31,4 +60,4 @@ Lemma wp_newServer :
     "#His_sigPk" ∷ is_sig_pk sigPk (serv_sigpred γ)
   }}}.
 Proof. Admitted.
-End specs.
+End wps.
